NuPrim.thy
@@ -9,16 +9,16 @@ theory NuPrim \<comment> \<open>The Primary Theory of the \<nu>-System\<close>
       and "with" = "\<^bold>w\<^bold>i\<^bold>t\<^bold>h"
       and "auxiliary_facts" = "\<^bold>w\<^bold>i\<^bold>t\<^bold>h \<^bold>f\<^bold>a\<^bold>c\<^bold>t\<^bold>s"
       and "auxfacts" = "\<^bold>w\<^bold>i\<^bold>t\<^bold>h \<^bold>f\<^bold>a\<^bold>c\<^bold>t\<^bold>s"
-      and "proc" = "\<^bold>p\<^bold>r\<^bold>o\<^bold>c"
-      and "map" = "\<^bold>m\<^bold>a\<^bold>p"
-      and "param" = "\<^bold>p\<^bold>a\<^bold>r\<^bold>a\<^bold>m"
+      and "<proc>" = "\<^bold>p\<^bold>r\<^bold>o\<^bold>c"
+      and "<map>" = "\<^bold>m\<^bold>a\<^bold>p"
+      and "<param>" = "\<^bold>p\<^bold>a\<^bold>r\<^bold>a\<^bold>m"
       and ",," = "\<heavy_comma>"
-      and cast = "\<^bold>c\<^bold>a\<^bold>s\<^bold>t"
-      and meanwhile = "\<^bold>m\<^bold>e\<^bold>a\<^bold>n\<^bold>w\<^bold>h\<^bold>i\<^bold>l\<^bold>e"
+      and "<cast>" = "\<^bold>c\<^bold>a\<^bold>s\<^bold>t"
+      and "<meanwhile>" = "\<^bold>m\<^bold>e\<^bold>a\<^bold>n\<^bold>w\<^bold>h\<^bold>i\<^bold>l\<^bold>e"
       and address = "\<^bold>a\<^bold>d\<^bold>d\<^bold>r\<^bold>e\<^bold>s\<^bold>s"
-      and conversion = "\<^bold>c\<^bold>o\<^bold>n\<^bold>v\<^bold>e\<^bold>r\<^bold>s\<^bold>i\<^bold>o\<^bold>n"
-      and auto = "\<^bold>a\<^bold>u\<^bold>t\<^bold>o"
-      and premise = "\<^bold>p\<^bold>r\<^bold>e\<^bold>m\<^bold>i\<^bold>s\<^bold>e"
+      and "<conversion>" = "\<^bold>c\<^bold>o\<^bold>n\<^bold>v\<^bold>e\<^bold>r\<^bold>s\<^bold>i\<^bold>o\<^bold>n"
+      and "<auto>" = "\<^bold>a\<^bold>u\<^bold>t\<^bold>o"
+      and "<premise>" = "\<^bold>p\<^bold>r\<^bold>e\<^bold>m\<^bold>i\<^bold>s\<^bold>e"
       and atomic = "\<^bold>a\<^bold>t\<^bold>o\<^bold>m\<^bold>i\<^bold>c"
       and construct = "\<^bold>c\<^bold>o\<^bold>n\<^bold>s\<^bold>t\<^bold>r\<^bold>u\<^bold>c\<^bold>t"
       and "by" = "\<^bold>b\<^bold>y"
@@ -246,19 +246,26 @@ lemma ParamTag: "\<^bold>p\<^bold>a\<^bold>r\<^bold>a\<^bold>m x" for x :: "'a" 
   \<comment>\<open>A tag used to indicate a parameter should be specified during application. It retains the order of the parameters to be specified.
   For example, "@{prop "\<And>bit_width value. \<^bold>p\<^bold>a\<^bold>r\<^bold>a\<^bold>m bit_width \<Longrightarrow> \<^bold>p\<^bold>a\<^bold>r\<^bold>a\<^bold>m value \<Longrightarrow> P bit_wdith value"},
     the first parameter `?bit_width` will be specified first and then the "?value".\<close>
+lemma [elim]: "\<^bold>p\<^bold>a\<^bold>r\<^bold>a\<^bold>m x \<Longrightarrow> C \<Longrightarrow> C" by auto
+
+definition ParamHOL :: " 'a \<Rightarrow> bool" where "ParamHOL x = True"
+lemma ParamHOL: "Trueprop (ParamHOL x) \<equiv> \<^bold>p\<^bold>a\<^bold>r\<^bold>a\<^bold>m x" unfolding ParamTag_def ParamHOL_def .
 
 subsubsection \<open>Premise tag\<close>
 
 definition Premise :: "bool \<Rightarrow> prop" ("\<^bold>p\<^bold>r\<^bold>e\<^bold>m\<^bold>i\<^bold>s\<^bold>e _" [10] 9) where [\<nu>def]:"Premise \<equiv> Trueprop"
   \<comment> \<open>A tag to hint automatic provers to try to prove this proof obligation\<close>
-lemma [simp]: "\<^bold>p\<^bold>r\<^bold>e\<^bold>m\<^bold>i\<^bold>s\<^bold>e P \<equiv> Trueprop P"  unfolding Premise_def .
-lemma Premise_I: "P \<Longrightarrow> \<^bold>p\<^bold>r\<^bold>e\<^bold>m\<^bold>i\<^bold>s\<^bold>e P" by simp
-lemma Premise_E: "\<^bold>p\<^bold>r\<^bold>e\<^bold>m\<^bold>i\<^bold>s\<^bold>e P \<Longrightarrow> P" by simp
-lemma Premise_Irew: "(P \<Longrightarrow> PROP C) \<equiv> (\<^bold>p\<^bold>r\<^bold>e\<^bold>m\<^bold>i\<^bold>s\<^bold>e P \<Longrightarrow> PROP C)" by simp
+lemma Premise_I: "P \<Longrightarrow> \<^bold>p\<^bold>r\<^bold>e\<^bold>m\<^bold>i\<^bold>s\<^bold>e P" unfolding Premise_def by simp
+lemma Premise_E: "\<^bold>p\<^bold>r\<^bold>e\<^bold>m\<^bold>i\<^bold>s\<^bold>e P \<Longrightarrow> P" unfolding Premise_def by simp
+lemma [elim]: "\<^bold>p\<^bold>r\<^bold>e\<^bold>m\<^bold>i\<^bold>s\<^bold>e P \<Longrightarrow> (P \<Longrightarrow> C) \<Longrightarrow> C" unfolding Premise_def by simp
+lemma Premise_Irew: "(P \<Longrightarrow> PROP C) \<equiv> (\<^bold>p\<^bold>r\<^bold>e\<^bold>m\<^bold>i\<^bold>s\<^bold>e P \<Longrightarrow> PROP C)" unfolding Premise_def by simp
 
-attribute_setup intro_premise = \<open>
+definition PremiseHOL :: "bool \<Rightarrow> bool" where "PremiseHOL x = x"
+lemma PremiseHOL: "Trueprop (PremiseHOL P) \<equiv> \<^bold>p\<^bold>r\<^bold>e\<^bold>m\<^bold>i\<^bold>s\<^bold>e P" unfolding Premise_def PremiseHOL_def .
+
+(* attribute_setup intro_premise = \<open>
   Scan.succeed (Thm.rule_attribute [] (fn _ => fn th => th COMP @{thm Premise_I}))
-\<close>
+\<close>*)
 attribute_setup elim_premise = \<open>
   Scan.succeed (Thm.rule_attribute [] (fn _ => fn th => th COMP @{thm Premise_E}))
 \<close>
@@ -649,7 +656,9 @@ lemma SpecTop_imp: "(PROP SpecTop (PROP P) (PROP L) \<Longrightarrow> PROP C) \<
   unfolding SpecTop_def conjunction_imp .
 lemma SpecTop_I: "PROP P \<Longrightarrow> PROP L \<Longrightarrow> PROP SpecTop (PROP P) (PROP L)" unfolding SpecTop_def using conjunctionI .
 
-lemma SpecTop_cong_major: "(P \<equiv> P') \<Longrightarrow> (P \<^bold>w\<^bold>i\<^bold>t\<^bold>h \<^bold>f\<^bold>a\<^bold>c\<^bold>t\<^bold>s: PROP Q) \<equiv> (P' \<^bold>w\<^bold>i\<^bold>t\<^bold>h \<^bold>f\<^bold>a\<^bold>c\<^bold>t\<^bold>s: PROP Q)"
+lemma SpecTop_cong_major:
+  "(P \<equiv> P') \<Longrightarrow> (PROP Q \<equiv> PROP Q') \<Longrightarrow>
+  (P \<^bold>w\<^bold>i\<^bold>t\<^bold>h \<^bold>f\<^bold>a\<^bold>c\<^bold>t\<^bold>s: PROP FactCollection (PROP Q) (PROP L) (PROP S)) \<equiv> (P' \<^bold>w\<^bold>i\<^bold>t\<^bold>h \<^bold>f\<^bold>a\<^bold>c\<^bold>t\<^bold>s: PROP FactCollection (PROP Q) (PROP L) (PROP S))"
     unfolding SpecTop_def by auto
 (*lemma Specification_rule_aux: "(P \<^bold>w\<^bold>i\<^bold>t\<^bold>h \<^bold>f\<^bold>a\<^bold>c\<^bold>t\<^bold>s: Q) \<Longrightarrow> (Q \<Longrightarrow> Q') \<Longrightarrow> (P \<^bold>w\<^bold>i\<^bold>t\<^bold>h \<^bold>f\<^bold>a\<^bold>c\<^bold>t\<^bold>s: Q')"
     unfolding SpecTop_def  by presburger *)
@@ -782,21 +791,26 @@ end
 definition AddtionTy :: " 'a set \<Rightarrow> bool \<Rightarrow> 'a set " (infixl "\<addition>" 50) where " T \<addition> P = {x. x \<in> T \<and> P}"
 lemma [simp]: "T \<addition> True = T" unfolding AddtionTy_def by fast
 lemma [simp]: "\<S_S> (T \<addition> P) = (\<S_S> T \<addition> P)" unfolding AddtionTy_def by auto
+lemma [simp]: "x \<in> (T \<addition> P) \<longleftrightarrow> x \<in> T \<and> P" unfolding AddtionTy_def by auto
 lemma [intro]: "P \<Longrightarrow> x \<in> T \<Longrightarrow> x \<in> (T \<addition> P)" unfolding AddtionTy_def by auto
 lemma [elim]: "x \<in> (T \<addition> P) \<Longrightarrow> (x \<in> T \<Longrightarrow> P \<Longrightarrow> C) \<Longrightarrow> C" unfolding AddtionTy_def by auto
-(* lemma [simp]: "((((\<^bold>c\<^bold>u\<^bold>r\<^bold>r\<^bold>e\<^bold>n\<^bold>t s \<^bold>r\<^bold>e\<^bold>s\<^bold>u\<^bold>l\<^bold>t\<^bold>s \<^bold>i\<^bold>n S) \<and> B) \<and> C) \<^bold>w\<^bold>i\<^bold>t\<^bold>h \<^bold>f\<^bold>a\<^bold>c\<^bold>t\<^bold>s: PROP L) \<equiv> (((\<^bold>c\<^bold>u\<^bold>r\<^bold>r\<^bold>e\<^bold>n\<^bold>t s \<^bold>r\<^bold>e\<^bold>s\<^bold>u\<^bold>l\<^bold>t\<^bold>s \<^bold>i\<^bold>n S) \<and> (B \<and> C)) \<^bold>w\<^bold>i\<^bold>t\<^bold>h \<^bold>f\<^bold>a\<^bold>c\<^bold>t\<^bold>s: PROP L)" by simp *)
+lemma [simp]: "(R \<heavy_comma> T \<addition> P) = ((R \<heavy_comma> T) \<addition> P)" and [simp]: "(A \<addition> P \<flower> B) = ((A \<flower> B) \<addition> P)"
+  and [simp]: "(A \<flower> B \<addition> P) = ((A \<flower> B) \<addition> P)"
+    unfolding AddtionTy_def by auto
+lemma [simp]: "(\<^bold>c\<^bold>u\<^bold>r\<^bold>r\<^bold>e\<^bold>n\<^bold>t s \<^bold>r\<^bold>e\<^bold>s\<^bold>u\<^bold>l\<^bold>t\<^bold>s \<^bold>i\<^bold>n T \<addition> P) \<longleftrightarrow> (\<^bold>c\<^bold>u\<^bold>r\<^bold>r\<^bold>e\<^bold>n\<^bold>t s \<^bold>r\<^bold>e\<^bold>s\<^bold>u\<^bold>l\<^bold>t\<^bold>s \<^bold>i\<^bold>n T) \<and> P" unfolding CurrentConstruction_def AddtionTy_def by (cases s) auto
+lemma [simp]: "((((\<^bold>c\<^bold>u\<^bold>r\<^bold>r\<^bold>e\<^bold>n\<^bold>t s \<^bold>r\<^bold>e\<^bold>s\<^bold>u\<^bold>l\<^bold>t\<^bold>s \<^bold>i\<^bold>n S) \<and> B) \<and> C) \<^bold>w\<^bold>i\<^bold>t\<^bold>h \<^bold>f\<^bold>a\<^bold>c\<^bold>t\<^bold>s: PROP L) \<equiv> (((\<^bold>c\<^bold>u\<^bold>r\<^bold>r\<^bold>e\<^bold>n\<^bold>t s \<^bold>r\<^bold>e\<^bold>s\<^bold>u\<^bold>l\<^bold>t\<^bold>s \<^bold>i\<^bold>n S) \<and> (B \<and> C)) \<^bold>w\<^bold>i\<^bold>t\<^bold>h \<^bold>f\<^bold>a\<^bold>c\<^bold>t\<^bold>s: PROP L)" by simp
 
-lemma t1: "(\<^bold>c\<^bold>u\<^bold>r\<^bold>r\<^bold>e\<^bold>n\<^bold>t s \<^bold>r\<^bold>e\<^bold>s\<^bold>u\<^bold>l\<^bold>t\<^bold>s \<^bold>i\<^bold>n T \<addition> P) \<longleftrightarrow> (\<^bold>c\<^bold>u\<^bold>r\<^bold>r\<^bold>e\<^bold>n\<^bold>t s \<^bold>r\<^bold>e\<^bold>s\<^bold>u\<^bold>l\<^bold>t\<^bold>s \<^bold>i\<^bold>n T) \<and> P" unfolding CurrentConstruction_def AddtionTy_def by (cases s) auto
-lemma [simp]:
-  "((\<^bold>c\<^bold>u\<^bold>r\<^bold>r\<^bold>e\<^bold>n\<^bold>t s \<^bold>r\<^bold>e\<^bold>s\<^bold>u\<^bold>l\<^bold>t\<^bold>s \<^bold>i\<^bold>n S \<addition> Q) \<^bold>w\<^bold>i\<^bold>t\<^bold>h \<^bold>f\<^bold>a\<^bold>c\<^bold>t\<^bold>s: PROP FactCollection (PROP NoFact) (PROP L) (PROP I))
-    \<equiv> (\<^bold>c\<^bold>u\<^bold>r\<^bold>r\<^bold>e\<^bold>n\<^bold>t s \<^bold>r\<^bold>e\<^bold>s\<^bold>u\<^bold>l\<^bold>t\<^bold>s \<^bold>i\<^bold>n S \<^bold>w\<^bold>i\<^bold>t\<^bold>h \<^bold>f\<^bold>a\<^bold>c\<^bold>t\<^bold>s: PROP FactCollection (Trueprop Q) (PROP L) (PROP I))"
-  unfolding t1 SpecTop_imp conj_imp FactCollection_imp
-  by (intro equal_intr_rule SpecTop_I FactCollection_I conjI NoFact) (unfold SpecTop_imp conj_imp FactCollection_imp)
-lemma [simp]:
-  "((\<^bold>c\<^bold>u\<^bold>r\<^bold>r\<^bold>e\<^bold>n\<^bold>t s \<^bold>r\<^bold>e\<^bold>s\<^bold>u\<^bold>l\<^bold>t\<^bold>s \<^bold>i\<^bold>n S \<addition> Q) \<^bold>w\<^bold>i\<^bold>t\<^bold>h \<^bold>f\<^bold>a\<^bold>c\<^bold>t\<^bold>s: PROP FactCollection (Trueprop P) (PROP L) (PROP I))
-    \<equiv> (\<^bold>c\<^bold>u\<^bold>r\<^bold>r\<^bold>e\<^bold>n\<^bold>t s \<^bold>r\<^bold>e\<^bold>s\<^bold>u\<^bold>l\<^bold>t\<^bold>s \<^bold>i\<^bold>n S \<^bold>w\<^bold>i\<^bold>t\<^bold>h \<^bold>f\<^bold>a\<^bold>c\<^bold>t\<^bold>s: PROP FactCollection  (Trueprop (Q \<and> P)) (PROP L) (PROP I))"
-  unfolding t1 SpecTop_imp conj_imp FactCollection_imp
-  by (intro equal_intr_rule SpecTop_I FactCollection_I conjI) (unfold SpecTop_imp conj_imp FactCollection_imp)
+
+lemma move_fact_to_star1[simp]:
+  "((\<^bold>c\<^bold>u\<^bold>r\<^bold>r\<^bold>e\<^bold>n\<^bold>t s \<^bold>r\<^bold>e\<^bold>s\<^bold>u\<^bold>l\<^bold>t\<^bold>s \<^bold>i\<^bold>n S) \<and> Q \<^bold>w\<^bold>i\<^bold>t\<^bold>h \<^bold>f\<^bold>a\<^bold>c\<^bold>t\<^bold>s: PROP FactCollection (PROP NoFact) (PROP L) (PROP I))
+    \<Longrightarrow> (\<^bold>c\<^bold>u\<^bold>r\<^bold>r\<^bold>e\<^bold>n\<^bold>t s \<^bold>r\<^bold>e\<^bold>s\<^bold>u\<^bold>l\<^bold>t\<^bold>s \<^bold>i\<^bold>n S \<^bold>w\<^bold>i\<^bold>t\<^bold>h \<^bold>f\<^bold>a\<^bold>c\<^bold>t\<^bold>s: PROP FactCollection (Trueprop Q) (PROP L) (PROP I))"
+  unfolding SpecTop_imp conj_imp FactCollection_imp
+  by (intro equal_intr_rule SpecTop_I FactCollection_I conjI NoFact) (* (unfold SpecTop_imp conj_imp FactCollection_imp) *)
+lemma move_fact_to_star2[simp]:
+  "((\<^bold>c\<^bold>u\<^bold>r\<^bold>r\<^bold>e\<^bold>n\<^bold>t s \<^bold>r\<^bold>e\<^bold>s\<^bold>u\<^bold>l\<^bold>t\<^bold>s \<^bold>i\<^bold>n S) \<and> Q \<^bold>w\<^bold>i\<^bold>t\<^bold>h \<^bold>f\<^bold>a\<^bold>c\<^bold>t\<^bold>s: PROP FactCollection (Trueprop P) (PROP L) (PROP I))
+    \<Longrightarrow> (\<^bold>c\<^bold>u\<^bold>r\<^bold>r\<^bold>e\<^bold>n\<^bold>t s \<^bold>r\<^bold>e\<^bold>s\<^bold>u\<^bold>l\<^bold>t\<^bold>s \<^bold>i\<^bold>n S \<^bold>w\<^bold>i\<^bold>t\<^bold>h \<^bold>f\<^bold>a\<^bold>c\<^bold>t\<^bold>s: PROP FactCollection  (Trueprop (Q \<and> P)) (PROP L) (PROP I))"
+  unfolding SpecTop_imp conj_imp FactCollection_imp
+  by (intro equal_intr_rule SpecTop_I FactCollection_I conjI) (* (unfold SpecTop_imp conj_imp FactCollection_imp) *)
 
   subsubsection \<open>Cast\<close>
 
@@ -821,9 +835,15 @@ lemma [\<nu>intro]: "\<^bold>c\<^bold>a\<^bold>s\<^bold>t A \<longmapsto> A' \<^
 lemma LooseState_Cast[\<nu>intro]: "\<^bold>c\<^bold>a\<^bold>s\<^bold>t A \<longmapsto> B \<Longrightarrow> \<^bold>c\<^bold>a\<^bold>s\<^bold>t \<S> A \<longmapsto> \<S> B" unfolding \<nu>def Cast_def by auto
 lemma [\<nu>intro]: "\<^bold>c\<^bold>a\<^bold>s\<^bold>t A \<longmapsto> A' \<^bold>m\<^bold>e\<^bold>a\<^bold>n\<^bold>w\<^bold>h\<^bold>i\<^bold>l\<^bold>e P \<Longrightarrow> \<^bold>c\<^bold>a\<^bold>s\<^bold>t B \<longmapsto> B' \<^bold>m\<^bold>e\<^bold>a\<^bold>n\<^bold>w\<^bold>h\<^bold>i\<^bold>l\<^bold>e Q \<Longrightarrow> \<^bold>c\<^bold>a\<^bold>s\<^bold>t (A\<heavy_comma>B) \<longmapsto> (A'\<heavy_comma>B') \<^bold>m\<^bold>e\<^bold>a\<^bold>n\<^bold>w\<^bold>h\<^bold>i\<^bold>l\<^bold>e P \<and>Q"
   unfolding Cast_def by auto
+lemma [\<nu>intro]: "\<^bold>c\<^bold>a\<^bold>s\<^bold>t A \<longmapsto> A' \<^bold>m\<^bold>e\<^bold>a\<^bold>n\<^bold>w\<^bold>h\<^bold>i\<^bold>l\<^bold>e P \<Longrightarrow> \<^bold>c\<^bold>a\<^bold>s\<^bold>t B \<longmapsto> B' \<^bold>m\<^bold>e\<^bold>a\<^bold>n\<^bold>w\<^bold>h\<^bold>i\<^bold>l\<^bold>e Q \<Longrightarrow> \<^bold>c\<^bold>a\<^bold>s\<^bold>t (A \<flower> B) \<longmapsto> (A' \<flower> B') \<^bold>m\<^bold>e\<^bold>a\<^bold>n\<^bold>w\<^bold>h\<^bold>i\<^bold>l\<^bold>e P \<and> Q"
+  unfolding Cast_def by auto
+lemma [\<nu>intro]: "\<^bold>c\<^bold>a\<^bold>s\<^bold>t A \<longmapsto> A' \<^bold>m\<^bold>e\<^bold>a\<^bold>n\<^bold>w\<^bold>h\<^bold>i\<^bold>l\<^bold>e P \<Longrightarrow> \<^bold>c\<^bold>a\<^bold>s\<^bold>t B \<longmapsto> B' \<^bold>m\<^bold>e\<^bold>a\<^bold>n\<^bold>w\<^bold>h\<^bold>i\<^bold>l\<^bold>e Q \<Longrightarrow> \<^bold>c\<^bold>a\<^bold>s\<^bold>t (A and_ty B) \<longmapsto> (A' and_ty B') \<^bold>m\<^bold>e\<^bold>a\<^bold>n\<^bold>w\<^bold>h\<^bold>i\<^bold>l\<^bold>e P \<and> Q"
+  unfolding Cast_def by auto
 
 theorem apply_cast: "(\<^bold>c\<^bold>u\<^bold>r\<^bold>r\<^bold>e\<^bold>n\<^bold>t blk \<^bold>r\<^bold>e\<^bold>s\<^bold>u\<^bold>l\<^bold>t\<^bold>s \<^bold>i\<^bold>n (R \<heavy_comma> X \<flower> W)) \<Longrightarrow> (\<^bold>c\<^bold>a\<^bold>s\<^bold>t X \<longmapsto> Y \<^bold>m\<^bold>e\<^bold>a\<^bold>n\<^bold>w\<^bold>h\<^bold>i\<^bold>l\<^bold>e P) \<Longrightarrow> (\<^bold>c\<^bold>u\<^bold>r\<^bold>r\<^bold>e\<^bold>n\<^bold>t blk \<^bold>r\<^bold>e\<^bold>s\<^bold>u\<^bold>l\<^bold>t\<^bold>s \<^bold>i\<^bold>n (R \<heavy_comma> Y \<flower> W) \<addition> P)"
   unfolding Procedure_def CurrentConstruction_def PendingConstruction_def bind_def SpecTop_imp by (auto 4 6)
+theorem cast: "\<^bold>c\<^bold>u\<^bold>r\<^bold>r\<^bold>e\<^bold>n\<^bold>t blk \<^bold>r\<^bold>e\<^bold>s\<^bold>u\<^bold>l\<^bold>t\<^bold>s \<^bold>i\<^bold>n T \<Longrightarrow> \<^bold>c\<^bold>a\<^bold>s\<^bold>t T \<longmapsto> T' \<^bold>m\<^bold>e\<^bold>a\<^bold>n\<^bold>w\<^bold>h\<^bold>i\<^bold>l\<^bold>e P \<Longrightarrow> \<^bold>c\<^bold>u\<^bold>r\<^bold>r\<^bold>e\<^bold>n\<^bold>t blk \<^bold>r\<^bold>e\<^bold>s\<^bold>u\<^bold>l\<^bold>t\<^bold>s \<^bold>i\<^bold>n T' "
+  for T' :: "('a::lrep) set" unfolding Cast_def CurrentConstruction_def by auto
 
 subsubsection \<open>Conversion\<close>
 
@@ -836,10 +856,10 @@ definition Conversion :: "( ('a::lrep) \<Rightarrow> ('b::lrep) state) \<Rightar
 lemma conversion: "\<^bold>c\<^bold>o\<^bold>n\<^bold>v\<^bold>e\<^bold>r\<^bold>s\<^bold>i\<^bold>o\<^bold>n f \<blangle> U \<longmapsto> V \<brangle> \<long_dobule_mapsto> f' \<blangle> U' \<longmapsto> V' \<brangle> \<Longrightarrow> \<^bold>p\<^bold>r\<^bold>o\<^bold>c f \<blangle> U \<longmapsto> V \<brangle> \<Longrightarrow> \<^bold>p\<^bold>r\<^bold>o\<^bold>c f' \<blangle> U' \<longmapsto> V' \<brangle>"
   for f :: " ('a::lrep) \<Rightarrow> ('b::lrep) state" and f' :: " ('c::lrep) \<Rightarrow> ('d::lrep) state" unfolding Conversion_def by fast
 lemma [\<nu>intro]: "\<^bold>c\<^bold>o\<^bold>n\<^bold>v\<^bold>e\<^bold>r\<^bold>s\<^bold>i\<^bold>o\<^bold>n f \<blangle> U \<longmapsto> V \<brangle> \<long_dobule_mapsto> f \<blangle> U \<longmapsto> V \<brangle>" unfolding Conversion_def by fast
-lemma [\<nu>intro]: "\<^bold>c\<^bold>o\<^bold>n\<^bold>v\<^bold>e\<^bold>r\<^bold>s\<^bold>i\<^bold>o\<^bold>n f \<blangle> U \<longmapsto> V \<brangle> \<long_dobule_mapsto> g \<blangle> U' \<longmapsto> V' \<brangle> \<Longrightarrow> \<^bold>c\<^bold>o\<^bold>n\<^bold>v\<^bold>e\<^bold>r\<^bold>s\<^bold>i\<^bold>o\<^bold>n f \<blangle> U \<longmapsto> V \<brangle> \<long_dobule_mapsto> call g \<blangle> U' \<flower> W \<longmapsto> V' \<flower> W\<brangle>"
-  unfolding Conversion_def using call by fast
 lemma [\<nu>intro]: "\<^bold>c\<^bold>a\<^bold>s\<^bold>t U' \<longmapsto> U \<^bold>m\<^bold>e\<^bold>a\<^bold>n\<^bold>w\<^bold>h\<^bold>i\<^bold>l\<^bold>e P \<Longrightarrow> \<^bold>c\<^bold>a\<^bold>s\<^bold>t V \<longmapsto> V' \<^bold>m\<^bold>e\<^bold>a\<^bold>n\<^bold>w\<^bold>h\<^bold>i\<^bold>l\<^bold>e Q \<Longrightarrow> \<^bold>c\<^bold>o\<^bold>n\<^bold>v\<^bold>e\<^bold>r\<^bold>s\<^bold>i\<^bold>o\<^bold>n f \<blangle> U \<longmapsto> V \<brangle> \<long_dobule_mapsto> f \<blangle> U' \<longmapsto> V'\<brangle>"
   unfolding Conversion_def Procedure_def Cast_def  by (auto 4 3 dest: LooseState_Cast[unfolded Cast_def, simplified])
+lemma [\<nu>intro]: "\<^bold>c\<^bold>o\<^bold>n\<^bold>v\<^bold>e\<^bold>r\<^bold>s\<^bold>i\<^bold>o\<^bold>n f \<blangle> U \<longmapsto> V \<brangle> \<long_dobule_mapsto> g \<blangle> U' \<longmapsto> V' \<brangle> \<Longrightarrow> \<^bold>c\<^bold>o\<^bold>n\<^bold>v\<^bold>e\<^bold>r\<^bold>s\<^bold>i\<^bold>o\<^bold>n f \<blangle> U \<longmapsto> V \<brangle> \<long_dobule_mapsto> call g \<blangle> U' \<flower> W \<longmapsto> V' \<flower> W\<brangle>"
+  unfolding Conversion_def using call by fast
 lemma [\<nu>intro]: "\<^bold>p\<^bold>r\<^bold>o\<^bold>c g \<blangle> U' \<longmapsto> U \<brangle> \<Longrightarrow> \<^bold>c\<^bold>o\<^bold>n\<^bold>v\<^bold>e\<^bold>r\<^bold>s\<^bold>i\<^bold>o\<^bold>n f \<blangle> U \<longmapsto> V \<brangle> \<long_dobule_mapsto> (g \<nuInstrComp> f) \<blangle> U' \<longmapsto> V\<brangle>"
   unfolding AutoTag_def Conversion_def using instr_comp by fast
 
@@ -866,6 +886,7 @@ lemma  [elim]: "(A\<heavy_comma>B) = (A'\<heavy_comma>B') \<Longrightarrow> (A =
 subsection \<open>Finalize the syntax sugars to be ready for use\<close>
 
 no_translations "_pretty_and_ P Q" <= "CONST AndFact P Q"
-(* translations "_linebreak_collection_ P Q" <= "CONST AndFact P Q" *)
+translations "_linebreak_collection_ P Q" <= "CONST AndFact P Q"
+translations "P" <= "CONST AndFact P (CONST NoFact)"
 
 end
